extracted inner while and added is_solution predicate

Licenta.dfy
@@ -1,6 +1,14 @@
-predicate valid_input(input: seq<int>)
+datatype Problem = Problem(number_of_objects: int, knapsack_capacity: int, costs: seq<int>, weights: seq<int>)
+
+predicate has_positive_values(input: seq<int>)
 {
-    forall i :: 0 <= i < |input| ==> input[i] >= 0
+    forall i :: 0 <= i < |input| ==> input[i] > 0
+}
+
+predicate is_valid_problem(p: Problem)
+{
+    |p.costs| == |p.weights| == p.number_of_objects && p.number_of_objects > 0 && p.knapsack_capacity > 0 && 
+          has_positive_values(p.costs) && has_positive_values(p.weights)
 }
 
 function max(p1: int, p2: int): int
@@ -8,13 +16,30 @@ function max(p1: int, p2: int): int
     if p1 > p2 then p1 else p2
 }
 
-// predicate is_solution(capacity: int, profit: int)
+function gain(s: seq<int>, c: seq<int>): int
+  requires |s| == |c| 
+{
+  if |s| == 0 then 0 else s[0] * c[0] + gain(s[1..], c[1..])
+}
+
+predicate is_solution(p: Problem, solution: seq<int>, profit: int)
+  requires |solution| == |p.costs| 
+{
+  gain(solution, p.costs) == profit
+}
+
+// predicate is_partial_solution(capacity: int, profit: int)
 // {
 
 // }
 
+predicate is_optimal_solution(p: Problem, solution: seq<int>, profit: int)
+  requires |solution| == |p.costs| 
+{
+    is_solution(p, solution, profit) // && orice alta solutie are gain < profit
+}
+
 method add_sequence(existing_seq: seq<seq<int>>, new_seq: seq<int>, c: int) returns (result: seq<seq<int>>)
-  requires |new_seq| > 0
   requires |new_seq| == c
   ensures result == existing_seq + [new_seq]
   ensures |result| == |existing_seq| + 1
@@ -22,58 +47,95 @@ method add_sequence(existing_seq: seq<seq<int>>, new_seq: seq<int>, c: int) retu
   result := existing_seq + [new_seq];
 }
 
-method get_maxim_profit(n: int, capacity: int, c: seq<int>, w: seq<int>) returns (maxim_profit : int)
-  requires n >= 0
-  requires capacity >= 0
-  requires valid_input(w)
-  requires valid_input(c)
-  requires n == |w| == |c|
+method get_maxim_profit(p: Problem) returns (maxim_profit : int, profits: seq<seq<int>>, solution: seq<int>)
+  requires is_valid_problem(p)
+  ensures |profits| == p.number_of_objects + 1
+  ensures forall k :: 0 <= k <= p.number_of_objects ==> |profits[k]| == p.knapsack_capacity + 1
+  // ensures is_solution(p, solution)
 {
-    var profits: seq<seq<int>> := []; 
+    profits := []; 
     maxim_profit := 0;
     
     var i := 0;
-    while i <= n 
-      invariant 0 <= i <= n + 1
+    while i <= p.number_of_objects 
+      invariant 0 <= i <= p.number_of_objects + 1
       invariant |profits| == i
-      invariant forall k :: 0 <= k < i ==> |profits[k]| == capacity + 1
+      invariant forall k :: 0 <= k < i ==> |profits[k]| == p.knapsack_capacity + 1
     {
-        var line: seq<int> := [];
-        var j := 0;
-        while j <= capacity
-          invariant 0 <= j <= capacity + 1
-          invariant 0 <= i <= n + 1 
-          invariant |line| == j
-          invariant forall k :: 0 <= k < i ==> |profits[k]| == capacity + 1
+        var partial_profits := get_partial_profits(p, profits,i);
+        profits := add_sequence(profits, partial_profits, p.knapsack_capacity + 1);
+        i := i + 1;
+    }
 
+    maxim_profit := profits[p.number_of_objects][p.knapsack_capacity];
+
+    solution := get_knapsack_objects(p, profits, maxim_profit);
+}
+
+method get_partial_profits(p: Problem, profits: seq<seq<int>>, i: int) returns (partial_profits: seq<int>)
+  requires is_valid_problem(p)
+  requires |profits| == i
+  requires 0 <= i < p.number_of_objects + 1
+  requires forall k :: 0 <= k < i ==> |profits[k]| == p.knapsack_capacity + 1
+  ensures |partial_profits| == p.knapsack_capacity + 1
+{
+        partial_profits := [];
+        var j := 0;
+        while j <= p.knapsack_capacity
+          invariant 0 <= i <= p.number_of_objects + 1 
+          invariant 0 <= j <= p.knapsack_capacity + 1
+          invariant |partial_profits| == j
         {
           if i == 0 || j == 0 {
-              line := line + [0];
+              partial_profits := partial_profits + [0];
           } else {
-            if w[i - 1] <= j {
-              line := line + [max(c[i - 1] + profits[i - 1][j - w[i - 1]], profits[i - 1][j])];
+            if p.weights[i - 1] <= j {
+              partial_profits := partial_profits + [max(p.costs[i - 1] + profits[i - 1][j - p.weights[i - 1]], profits[i - 1][j])];
             } else {
-              line := line + [profits[i - 1][j]];
+              partial_profits := partial_profits + [profits[i - 1][j]];
             }
           }
           j := j + 1;
         }
-        profits := add_sequence(profits, line, capacity + 1);
-        i := i + 1;
-    }
+}
 
-    maxim_profit := profits[n][capacity];
+method get_knapsack_objects(p: Problem, profits: seq<seq<int>>, maxim_profit: int) returns (solution: seq<int>)
+  requires is_valid_problem(p)
+  requires |profits| == p.number_of_objects + 1
+  requires forall k :: 0 <= k <= p.number_of_objects ==> |profits[k]| == p.knapsack_capacity + 1
+  ensures |solution| == p.number_of_objects == |p.weights| == |p.costs|
+  // ensures is_solution(p, solution)
+{
+    solution := [];
+    var i := p.number_of_objects;
+    var j := p.knapsack_capacity;
+
+    while i > 0 && j >= 0
+      invariant 0 <= i <= p.number_of_objects
+      invariant 0 <= j <= p.knapsack_capacity
+      invariant |solution| == p.number_of_objects - i
+      decreases i
+      decreases j
+    {
+      if profits[i][j] == profits[i - 1][j] {
+        solution := [0] + solution;
+        i := i - 1;
+      } else { 
+        solution := [1] + solution;
+        i := i - 1;
+        if j - p.weights[i] >= 0 {
+          j := j - p.weights[i];
+        }
+        
+      }
+    }
+    assert |solution| == |p.weights|;
 }
 
 method Main()
 {
-    var number_of_objects: int := 4; 
-    var knapsack_capacity: int := 8;
-
-    var costs := [1, 2, 5, 6];
-    var weights := [2, 3, 4, 5];
-
-    var maxim_profit := get_maxim_profit(number_of_objects, knapsack_capacity, costs, weights);
+    var problem: Problem := Problem(number_of_objects := 4, knapsack_capacity := 8, costs := [1, 2, 5, 6], weights := [2, 3, 4, 5]);
+    var maxim_profit, profits, solution := get_maxim_profit(problem);
 
     print "Maxim profit: ";
     print maxim_profit;
